non-cps

theories/input_lang_callcc/interp.v
@@ -24,7 +24,7 @@ Program Definition callccE : opInterp :=  {|
 
 Program Definition throwE : opInterp :=  {|
                                          Ins := (▶ ∙ * (▶ (∙ -n> ∙)));
-                                         Outs := unitO;
+                                         Outs := Empty_setO;
                                        |}.
 
 Definition ioE := @[inputE;outputE;callccE;throwE].
@@ -51,7 +51,7 @@ Proof.
     + apply Hs'.
   - simple refine (λne (us : prodO (prodO ((laterO X -n> laterO X) -n> laterO X) stateO) (laterO X -n> laterO X)), Some $ ((fstO (fstO us)) (sndO us), sndO (fstO us))).
     solve_proper.
-  - simple refine (λne (us : prodO (prodO (prodO (laterO X) (laterO (X -n> X))) stateO) (unitO -n> laterO X)), Some (laterO_ap us.1.1.2 us.1.1.1, sndO (fstO us))).
+  - simple refine (λne (us : prodO (prodO (prodO (laterO X) (laterO (X -n> X))) stateO) (Empty_setO -n> laterO X)), Some (laterO_ap us.1.1.2 us.1.1.1, sndO (fstO us))).
     intros ????.
     repeat f_equiv; assumption.
 Defined.
@@ -63,34 +63,11 @@ Section constructors.
   Notation IT := (IT E A).
   Notation ITV := (ITV E A).
 
-  Program Definition CALLCC : ((laterO IT -n> laterO IT) -n> laterO IT) -n> (laterO IT -n> laterO IT) -n> IT :=
-    λne e k, Vis (E:=E) (subEff_opid (inr (inr (inl ()))))
-               (subEff_ins (F:=ioE) (op:=(inr (inr (inl ())))) e)
-               (λne o, (k ((subEff_outs (F:=ioE) (op:=(inr (inr (inl ())))))^-1 o))).
-  Next Obligation.
-    intros.
-    intros ???.
-    by do 2 f_equiv.
-  Qed.
-  Next Obligation.
-    intros.
-    intros ???.
-    f_equiv.
-    intros ?; simpl.
-    by do 1 f_equiv.
-  Qed.
-  Next Obligation.
-    intros ?????; simpl.
-    by do 2 f_equiv.
-  Qed.
-
-  Lemma hom_CALLCC e k f `{!IT_hom f} : f (CALLCC e k) ≡ CALLCC e (laterO_map (OfeMor f) ◎ k).
-  Proof.
-    unfold CALLCC.
-    rewrite hom_vis/=. repeat f_equiv.
-    intro x. cbn-[laterO_map].
-    f_equiv.
-  Qed.
+  Program Definition CALLCC : ((laterO IT -n> laterO IT) -n> laterO IT) -n> IT :=
+    λne k, Vis (E:=E) (subEff_opid (inr (inr (inl ()))))
+             (subEff_ins (F:=ioE) (op:=(inr (inr (inl ())))) k)
+             (λne o, (subEff_outs (F:=ioE) (op:=(inr (inr (inl ())))))^-1 o).
+  Solve All Obligations with solve_proper.
 
   Program Definition INPUT : (nat -n> IT) -n> IT := λne k, Vis (E:=E) (subEff_opid (inl ()))
                                                              (subEff_ins (F:=ioE) (op:=(inl ())) ())
@@ -184,59 +161,7 @@ Section weakestpre.
     { simpl. done. }
     iModIntro. iIntros "H1 H2".
     iApply wp_val. by iApply ("Ha" with "H1 H2").
-    Unshelve.
-    simpl; constructor.
-  Qed.
-
-  (* wp_subreify *)
-  (* Lemma wp_callcc (σ : stateO) (e : (laterO IT -n> laterO IT) -n> laterO IT) (k : laterO IT -n> laterO IT) Φ s : *)
-  (*   has_substate σ -∗ *)
-  (*   ▷ (£ 1 -∗ has_substate σ -∗ WP@{rs} (later_car (k (e k))) @ s {{ Φ }}) -∗ *)
-  (*   WP@{rs} (CALLCC e k) @ s {{ Φ }}. *)
-  (* Proof. *)
-  (*   iIntros "Hs Ha". *)
-  (*   unfold CALLCC. simpl. *)
-  (*   iApply (wp_subreify with "Hs"). *)
-  (*   { *)
-  (*     simpl. *)
-  (*     do 2 f_equiv; last reflexivity. *)
-  (*     Unshelve. *)
-  (*     3: apply (k (e k)). *)
-  (*     2: simpl; apply (e k). *)
-  (*     simpl. *)
-  (*     rewrite ofe_iso_21. *)
-  (*     admit. *)
-  (*   } *)
-  (*   { *)
-  (*     simpl. *)
-  (*     rewrite ofe_iso_21. *)
-  (*     f_equiv. *)
-  (*   } *)
-  (*   iModIntro. *)
-  (*   iApply "Ha". *)
-  (* Admitted. *)
-
-  Lemma wp_throw (σ : stateO) (f : laterO (IT -n> IT)) (x : IT) Φ s :
-    has_substate σ -∗
-    ▷ (£ 1 -∗ has_substate σ -∗ WP@{rs} later_car f x @ s {{ Φ }}) -∗
-    WP@{rs} (THROW x f) @ s {{ Φ }}.
-  Proof.
-    iIntros "Hs Ha".
-    unfold THROW. simpl.
-    iApply (wp_subreify with "Hs").
-    {
-      simpl.
-      do 2 f_equiv; reflexivity.
-    }
-    {
-      simpl.
-      reflexivity.
-    }
-    iModIntro.
-    iApply "Ha".
-    Unshelve.
-    simpl.
-    constructor.
+    Unshelve. simpl; constructor.
   Qed.
 
 End weakestpre.
@@ -245,455 +170,158 @@ Section interp.
   Context {sz : nat}.
   Variable (rs : gReifiers sz).
   Context {subR : subReifier reify_io rs}.
-  Context {R} `{!Cofe R}.
+  Context {R} `{CR : !Cofe R}.
   Context `{!SubOfe natO R}.
   Notation F := (gReifiers_ops rs).
   Notation IT := (IT F R).
   Notation ITV := (ITV F R).
 
   Context {subEff0 : subEff ioE F}.
-
   (** Interpreting individual operators *)
-  Program Definition interp_input {A} : A -n> (IT -n> IT) -n> IT :=
-    λne env κ, κ (INPUT Ret).
-  Solve All Obligations with solve_proper.
+  Program Definition interp_input {A} : A -n> IT :=
+    λne env, INPUT Ret.
+  Program Definition interp_output {A} (t : A -n> IT) : A -n> IT :=
+    get_ret OUTPUT ◎ t.
+  Local Instance interp_ouput_ne {A} : NonExpansive2 (@interp_output A).
+  Proof. solve_proper. Qed.
 
-  Program Definition interp_output {A} (t : A -n> (IT -n> IT) -n> IT) : A -n> (IT -n> IT) -n> IT :=
-    λne env κ, t env (λne x, κ ((get_ret OUTPUT x))).
-  Solve All Obligations with try solve_proper.
-  Next Obligation.
-    solve_proper_prepare.
-    repeat f_equiv.
-    intros ?; simpl.
-    by repeat f_equiv.
-  Qed.
-  Next Obligation.
-    solve_proper_prepare.
-    by repeat f_equiv.
-  Qed.
-
-  Program Definition interp_callcc {S} (e : @interp_scope F R _ (inc S) -n> (IT -n> IT) -n> IT)
-    : interp_scope S -n> (IT -n> IT) -n> IT := λne env κ, CALLCC (λne (f : laterO IT -n> laterO IT), f (Next (e (@extend_scope F R _ _ env (Fun (Next κ))) κ))) (laterO_ap (Next κ)).
+  Program Definition interp_callcc {S} (e : @interp_scope F R _ (inc S) -n> IT)
+    : interp_scope S -n> IT := λne env, CALLCC (λne (f : laterO IT -n> laterO IT), (Next (e (@extend_scope F R _ _ env (Fun (Next (λne x, Tau (f (Next x))))))))).
   Next Obligation.
     solve_proper.
   Qed.
   Next Obligation.
-    intros; intros ???.
+    solve_proper_prepare.
     repeat f_equiv.
-    - intros a; simpl.
-      repeat f_equiv; [| assumption].
-      intros [| ?]; simpl; solve_proper.
-    - assumption.
+    intros [| a]; simpl; last solve_proper.
+    repeat f_equiv.
+    intros ?; simpl.
+    by repeat f_equiv.
   Qed.
   Next Obligation.
-    intros; intros ????; simpl.
-    repeat f_equiv; intros ?; simpl.
+    solve_proper_prepare.
     repeat f_equiv.
-    intros [| ?]; simpl; solve_proper.
+    intros ?; simpl.
+    repeat f_equiv.
+    intros [| a]; simpl; last solve_proper.
+    repeat f_equiv.
   Qed.
 
-  Program Definition interp_throw {A} (n : A -n> (IT -n> IT) -n> IT) (m : A -n> (IT -n> IT) -n> IT)
-    : A -n> (IT -n> IT) -n> IT := λne env κ, n env (λne n', m env (λne m', get_fun (λne (f : laterO (IT -n> IT)), THROW n' f) m')).
+  Program Definition interp_throw {A} (n : A -n> IT) (m : A -n> IT)
+    : A -n> IT := λne env, get_fun (λne (f : laterO (IT -n> IT)), THROW (n env) f) (m env).
   Next Obligation.
-    intros ???????????.
+    intros ????.
+    intros n' x y H.
     f_equiv; assumption.
   Qed.
-  Next Obligation.
-    solve_proper_prepare.
-    repeat f_equiv; last done.
-  Qed.
-  Next Obligation.
-    solve_proper_prepare.
-    repeat f_equiv.
-    intros ?; simpl.
-    repeat f_equiv.
-    intros ?; simpl.
-    repeat f_equiv; first done.
-    intros ?; simpl.
-    by repeat f_equiv.
-  Qed.
-  Next Obligation.
-    solve_proper_prepare.
-    repeat f_equiv.
-  Qed.
-  Next Obligation.
-    solve_proper_prepare.
-    repeat f_equiv; first done.
-    intros ?; simpl.
-    by repeat f_equiv.
-  Qed.
 
-  Global Instance interp_throw_ne A : NonExpansive2 (@interp_throw A).
-  Proof.
-    solve_proper_prepare.
-    repeat f_equiv; first done.
-    intros ?; simpl.
-    repeat f_equiv; first done.
-  Qed.
-  Typeclasses Opaque interp_throw.
-
-  Program Definition interp_natop {A} (op : nat_op) (t1 t2 : A -n> (IT -n> IT) -n> IT) : A -n> (IT -n> IT) -n> IT :=
-    λne env κ, (t1 env (λne n, t2 env (λne m, κ (NATOP (do_natop op) n m)))).
-  Solve All Obligations with try solve_proper.
-  Next Obligation.
-    solve_proper_prepare.
-    f_equiv.
-    intros ?; simpl.
-    by repeat f_equiv.
-  Qed.
-  Next Obligation.
-    solve_proper_prepare.
-    repeat f_equiv.
-    intros ?; simpl.
-    repeat f_equiv.
-    intros ?; simpl.
-    by repeat f_equiv.
-  Qed.
-  Next Obligation.
-    solve_proper_prepare.
-    repeat f_equiv; first done.
-    intros ?; simpl.
-    by repeat f_equiv.
-  Qed.
+  Program Definition interp_natop {A} (op : nat_op) (t1 t2 : A -n> IT) : A -n> IT :=
+    λne env, NATOP (do_natop op) (t1 env) (t2 env).
+  Solve All Obligations with solve_proper_please.
 
   Global Instance interp_natop_ne A op : NonExpansive2 (@interp_natop A op).
-  Proof.
-    solve_proper_prepare.
-    repeat f_equiv; first done.
-    intros ?; simpl.
-    by repeat f_equiv.
-  Qed.
+  Proof. solve_proper. Qed.
   Typeclasses Opaque interp_natop.
 
   Opaque laterO_map.
+  Program Definition interp_rec_pre {S : Set} (body : @interp_scope F R _ (inc (inc S)) -n> IT)
+    : laterO (@interp_scope F R _ S -n> IT) -n> @interp_scope F R _ S -n> IT :=
+    λne self env, Fun $ laterO_map (λne (self : @interp_scope F R  _ S -n> IT) (a : IT),
+                      body (@extend_scope F R _ _ (@extend_scope F R _ _ env (self env)) a)) self.
+  Next Obligation.
+    intros.
+    solve_proper_prepare.
+    f_equiv; intros [| [| y']]; simpl; solve_proper.
+  Qed.
+  Next Obligation.
+    intros.
+    solve_proper_prepare.
+    f_equiv; intros [| [| y']]; simpl; solve_proper.
+  Qed.
+  Next Obligation.
+    intros.
+    solve_proper_prepare.
+    do 3 f_equiv; intros ??; simpl; f_equiv;
+    intros [| [| y']]; simpl; solve_proper.
+  Qed.
+  Next Obligation.
+    intros.
+    solve_proper_prepare.
+    by do 2 f_equiv.
+  Qed.
 
-  Program Definition interp_app {A} (t1 t2 : A -n> (IT -n> IT) -n> IT) : A -n> (IT -n> IT) -n> IT :=
-    λne env κ, t1 env (λne m, t2 env (λne n, κ (APP' m n))).
+  Program Definition interp_rec {S : Set} (body : @interp_scope F R _ (inc (inc S)) -n> IT) : @interp_scope F R _ S -n> IT := mmuu (interp_rec_pre body).
+
+  Program Definition ir_unf {S : Set} (body : @interp_scope F R _ (inc (inc S)) -n> IT) env : IT -n> IT :=
+    λne a, body (@extend_scope F R _ _ (@extend_scope F R _ _ env (interp_rec body env)) a).
   Next Obligation.
-    solve_proper.
-  Qed.
-  Next Obligation.
-    solve_proper_please.
-  Qed.
-  Next Obligation.
-    intros; intros ???.
-    f_equiv; intros ?; simpl.
-    f_equiv; intros ?; simpl.
-    by f_equiv.
-  Qed.
-  Next Obligation.
-    solve_proper_please.
+    intros.
+    solve_proper_prepare.
+    f_equiv. intros [| [| y']]; simpl; solve_proper.
   Qed.
 
+  Lemma interp_rec_unfold {S : Set} (body : @interp_scope F R _ (inc (inc S)) -n> IT) env :
+    interp_rec body env ≡ Fun $ Next $ ir_unf body env.
+  Proof.
+    trans (interp_rec_pre body (Next (interp_rec body)) env).
+    { f_equiv. rewrite /interp_rec. apply mmuu_unfold. }
+    simpl. rewrite laterO_map_Next. repeat f_equiv.
+    simpl. unfold ir_unf. intro. simpl. reflexivity.
+  Qed.
+
+  Program Definition interp_app {A} (t1 t2 : A -n> IT) : A -n> IT :=
+    λne env, APP' (t1 env) (t2 env).
+  Solve All Obligations with first [ solve_proper | solve_proper_please ].
+  Global Instance interp_app_ne A : NonExpansive2 (@interp_app A).
+  Proof. solve_proper. Qed.
   Typeclasses Opaque interp_app.
 
-  Program Definition interp_if {A} (t0 t1 t2 : A -n> (IT -n> IT) -n> IT) : A -n> (IT -n> IT) -n> IT :=
-    λne env κ, (t0 env (λne b, (IF b (t1 env κ) (t2 env κ)))).
-  Solve All Obligations with try solve_proper.
-  Next Obligation.
-    solve_proper_prepare.
-    f_equiv.
-    intros ?; simpl; solve_proper.
-  Qed.
-  Next Obligation.
-    solve_proper_prepare.
-    repeat f_equiv; first done.
-    intros ?; simpl.
-    by repeat f_equiv.
-  Qed.
-
+  Program Definition interp_if {A} (t0 t1 t2 : A -n> IT) : A -n> IT :=
+    λne env, IF (t0 env) (t1 env) (t2 env).
+  Solve All Obligations with first [ solve_proper | solve_proper_please ].
   Global Instance interp_if_ne A n :
     Proper ((dist n) ==> (dist n) ==> (dist n) ==> (dist n)) (@interp_if A).
-  Proof.
-    solve_proper_prepare.
-    repeat f_equiv; first solve_proper.
-    intros ?; simpl.
-    repeat f_equiv; solve_proper.
-  Qed.
+  Proof. solve_proper. Qed.
 
-  Program Definition interp_nat (n : nat) {A} : A -n> (IT -n> IT) -n> IT :=
-    λne env κ, κ (Ret n).
+  Program Definition interp_nat (n : nat) {A} : A -n> IT :=
+    λne env, Ret n.
+
+  Program Definition interp_cont {A} (K : A -n> (IT -n> IT)) : A -n> IT := λne env, Fun (Next (K env)).
   Solve All Obligations with solve_proper.
 
-  Program Definition interp_var' {S : Set} (v : S) : interp_scope S -n> (IT -n> IT) -n> IT :=
-    λne (f : interp_scope S) κ, κ (interp_var v f).
+  Program Definition interp_applk {A} (q : A -n> IT) (K : A -n> (IT -n> IT)) : A -n> (IT -n> IT) := λne env t, interp_app q (λne env, K env t) env.
   Solve All Obligations with solve_proper.
 
-  Program Definition interp_emptyk {A} : (A -n> (IT -n> IT) -n> IT) -n> (A -n> (IT -n> IT) -n> IT) := λne φ env κ, φ env κ.
-  Solve All Obligations with try solve_proper.
+  Program Definition interp_apprk {A} (K : A -n> (IT -n> IT)) (q : A -n> IT) : A -n> (IT -n> IT) := λne env t, interp_app (λne env, K env t) q env.
+  Solve All Obligations with solve_proper.
 
-  Program Definition interp_outputk {A} (K : (A -n> (IT -n> IT) -n> IT) -n> (A -n> (IT -n> IT) -n> IT)) : (A -n> (IT -n> IT) -n> IT) -n> (A -n> (IT -n> IT) -n> IT) := λne φ env κ, interp_output (K φ) env κ.
-  Solve All Obligations with try solve_proper.
-  Next Obligation.
-    solve_proper_prepare.
-    repeat f_equiv.
-    intros ?; simpl.
-    by repeat f_equiv.
-  Qed.
-  Next Obligation.
-    solve_proper_prepare.
-    by repeat f_equiv.
-  Qed.
-  Next Obligation.
-    solve_proper_prepare.
-    by repeat f_equiv.
-  Qed.
+  Program Definition interp_natoplk {A} (op : nat_op) (q : A -n> IT) (K : A -n> (IT -n> IT)) : A -n> (IT -n> IT) := λne env t, interp_natop op q (λne env, K env t) env.
+  Solve All Obligations with solve_proper.
 
-  Program Definition interp_ifk {A} (K : (A -n> (IT -n> IT) -n> IT) -n> (A -n> (IT -n> IT) -n> IT))
-    (q : A -n> (IT -n> IT) -n> IT)
-    (p : A -n> (IT -n> IT) -n> IT)
-    : (A -n> (IT -n> IT) -n> IT) -n> (A -n> (IT -n> IT) -n> IT)
-    := λne φ env κ, interp_if (K φ) q p env κ.
-  Solve All Obligations with try solve_proper.
-  Next Obligation.
-    solve_proper_prepare.
-    repeat f_equiv.
-    intros ?; simpl.
-    by repeat f_equiv.
-  Qed.
-  Next Obligation.
-    solve_proper_prepare.
-    repeat f_equiv; first done.
-    intros ?; simpl.
-    by repeat f_equiv.
-  Qed.
-  Next Obligation.
-    solve_proper_prepare.
-    by repeat f_equiv.
-  Qed.
+  Program Definition interp_natoprk {A} (op : nat_op) (K : A -n> (IT -n> IT)) (q : A -n> IT) : A -n> (IT -n> IT) := λne env t, interp_natop op (λne env, K env t) q env.
+  Solve All Obligations with solve_proper.
 
-  Program Definition interp_applk {A} (q : A -n> (IT -n> IT) -n> IT)
-    (K : (A -n> (IT -n> IT) -n> IT) -n> (A -n> (IT -n> IT) -n> IT))
-    : (A -n> (IT -n> IT) -n> IT) -n> (A -n> (IT -n> IT) -n> IT)
-    := λne φ env κ, interp_app q (K φ) env κ.
-  Solve All Obligations with try solve_proper.
-  Next Obligation.
-    solve_proper_prepare.
-    repeat f_equiv.
-    intros ?; simpl.
-    repeat f_equiv.
-    intros ?; simpl.
-    by repeat f_equiv.
-  Qed.
-  Next Obligation.
-    solve_proper_prepare.
-    repeat f_equiv; first done.
-    intros ?; simpl.
-    by repeat f_equiv.
-  Qed.
-  Next Obligation.
-    solve_proper_prepare.
-    repeat f_equiv.
-    intros ?; simpl.
-    by repeat f_equiv.
-  Qed.
+  Program Definition interp_ifk {A} (K : A -n> (IT -n> IT)) (q : A -n> IT) (p : A -n> IT) : A -n> (IT -n> IT) := λne env t, interp_if (λne env, K env t) q p env.
+  Solve All Obligations with solve_proper.
 
-  Program Definition interp_apprk {A} (K : (A -n> (IT -n> IT) -n> IT) -n> (A -n> (IT -n> IT) -n> IT))
-    (q : A -n> (IT -n> IT) -n> IT)
-    : (A -n> (IT -n> IT) -n> IT) -n> (A -n> (IT -n> IT) -n> IT)
-    := λne φ env κ, interp_app (K φ) q env κ.
-  Solve All Obligations with try solve_proper.
-  Next Obligation.
-    solve_proper_prepare.
-    repeat f_equiv.
-    intros ?; simpl.
-    repeat f_equiv.
-    intros ?; simpl.
-    by repeat f_equiv.
-  Qed.
-  Next Obligation.
-    solve_proper_prepare.
-    repeat f_equiv; first done.
-    intros ?; simpl.
-    by repeat f_equiv.
-  Qed.
-  Next Obligation.
-    solve_proper_prepare.
-    by repeat f_equiv.
-  Qed.
+  Program Definition interp_outputk {A} (K : A -n> (IT -n> IT)) : A -n> (IT -n> IT) := λne env t, interp_output (λne env, K env t) env.
+  Solve All Obligations with solve_proper.
 
-  Program Definition interp_natoplk {A} (op : nat_op)
-    (q : A -n> (IT -n> IT) -n> IT)
-    (K : (A -n> (IT -n> IT) -n> IT) -n> (A -n> (IT -n> IT) -n> IT))
-    : (A -n> (IT -n> IT) -n> IT) -n> (A -n> (IT -n> IT) -n> IT)
-    := λne φ env κ, interp_natop op q (K φ) env κ.
-  Solve All Obligations with try solve_proper.
-  Next Obligation.
-    solve_proper_prepare.
-    repeat f_equiv.
-    intros ?; simpl.
-    repeat f_equiv.
-    intros ?; simpl.
-    by repeat f_equiv.
-  Qed.
-  Next Obligation.
-    solve_proper_prepare.
-    repeat f_equiv; first done.
-    intros ?; simpl.
-    by repeat f_equiv.
-  Qed.
-  Next Obligation.
-    solve_proper_prepare.
-    repeat f_equiv.
-    intros ?; simpl.
-    by repeat f_equiv.
-  Qed.
+  Program Definition interp_throwlk {A} (K : A -n> (IT -n> IT)) (q : A -n> IT) : A -n> (IT -n> IT) := λne env t, interp_throw (λne env, K env t) q env.
+  Solve All Obligations with solve_proper_please.
 
-  Program Definition interp_natoprk {A} (op : nat_op)
-    (K : (A -n> (IT -n> IT) -n> IT) -n> (A -n> (IT -n> IT) -n> IT))
-    (q : A -n> (IT -n> IT) -n> IT)
-    : (A -n> (IT -n> IT) -n> IT) -n> (A -n> (IT -n> IT) -n> IT)
-    := λne φ env κ, interp_natop op (K φ) q env κ.
-  Solve All Obligations with try solve_proper.
-  Next Obligation.
-    solve_proper_prepare.
-    repeat f_equiv.
-    intros ?; simpl.
-    repeat f_equiv.
-    intros ?; simpl.
-    by repeat f_equiv.
-  Qed.
-  Next Obligation.
-    solve_proper_prepare.
-    repeat f_equiv; first done.
-    intros ?; simpl.
-    by repeat f_equiv.
-  Qed.
-  Next Obligation.
-    solve_proper_prepare.
-    by repeat f_equiv.
-  Qed.
-
-  Program Definition interp_throwlk {A}
-    (K : (A -n> (IT -n> IT) -n> IT) -n> (A -n> (IT -n> IT) -n> IT))
-    (q : A -n> (IT -n> IT) -n> IT)
-    : (A -n> (IT -n> IT) -n> IT) -n> (A -n> (IT -n> IT) -n> IT)
-    := λne φ env κ, interp_throw (K φ) q env κ.
-  Solve All Obligations with try solve_proper.
-  Next Obligation.
-    solve_proper_prepare.
-    repeat f_equiv; first done.
-    intros ?; simpl.
-    by repeat f_equiv.
-  Qed.
-  Next Obligation.
-    solve_proper_prepare.
-    by repeat f_equiv.
-  Qed.
-
-  Program Definition interp_throwrk {A}
-    (q : A -n> (IT -n> IT) -n> IT)
-    (K : (A -n> (IT -n> IT) -n> IT) -n> (A -n> (IT -n> IT) -n> IT))
-    : (A -n> (IT -n> IT) -n> IT) -n> (A -n> (IT -n> IT) -n> IT)
-    := λne φ env κ, interp_throw q (K φ) env κ.
-  Solve All Obligations with try solve_proper.
-  Next Obligation.
-    solve_proper_prepare.
-    repeat f_equiv; first done.
-    intros ?; simpl.
-    by repeat f_equiv.
-  Qed.
-  Next Obligation.
-    solve_proper_prepare.
-    repeat f_equiv.
-    intros ?; simpl.
-    by repeat f_equiv.
-  Qed.
-
-  (* Wrong *)
-  Program Definition interp_rec_pre {S : Set} (body : @interp_scope F R _ (inc (inc S)) -n> (IT -n> IT) -n> IT)
-    : laterO (@interp_scope F R _ S -n> (IT -n> IT) -n> IT) -n> @interp_scope F R _ S -n> (IT -n> IT) -n> IT :=
-    λne self env κ,
-      κ (Fun $ laterO_map (λne
-                             (self : @interp_scope F R  _ S -n> (IT -n> IT) -n> IT)
-                             (a : IT),
-             body
-               (@extend_scope F R _ _ (@extend_scope F R _ _ env (self env κ)) a)
-               κ
-           ) self).
-  Next Obligation.
-    intros.
-    solve_proper_prepare.
-    do 2 f_equiv; intros [| [| y']]; simpl; solve_proper.
-  Qed.
-  Next Obligation.
-    intros.
-    solve_proper_prepare.
-    do 2 f_equiv; intros [| [| y']]; simpl; solve_proper.
-  Qed.
-  Next Obligation.
-    intros.
-    solve_proper_prepare.
-    f_equiv; [assumption |].
-    do 3 f_equiv; intros ??; simpl; f_equiv.
-    - f_equiv; intros [| [| y']]; simpl; solve_proper.
-    - assumption.
-  Qed.
-  Next Obligation.
-    intros.
-    solve_proper_prepare.
-    do 4 f_equiv; intros ??; simpl.
-    do 2 f_equiv; intros [| [| y']]; simpl; solve_proper.
-  Qed.
-  Next Obligation.
-    intros.
-    solve_proper_prepare.
-    by do 3 f_equiv.
-  Qed.
-
-  Program Definition interp_rec {S : Set} (body : @interp_scope F R _ (inc (inc S)) -n> (IT -n> IT) -n> IT) : @interp_scope F R _ S -n> (IT -n> IT) -n> IT := mmuu (interp_rec_pre body).
-
-  Program Definition ir_unf {S : Set} (body : @interp_scope F R _ (inc (inc S)) -n> (IT -n> IT) -n> IT) env κ : IT -n> IT :=
-    λne a, body (@extend_scope F R _ _ (@extend_scope F R _ _ env (interp_rec body env κ)) a) κ.
-  Next Obligation.
-    intros.
-    solve_proper_prepare.
-    repeat f_equiv; intros [| [| y']]; simpl; solve_proper.
-  Qed.
-
-  Lemma interp_rec_unfold {S : Set} (body : @interp_scope F R _ (inc (inc S)) -n> (IT -n> IT) -n> IT) env κ :
-    interp_rec body env κ ≡ κ $ Fun $ Next $ ir_unf body env κ.
-  Proof.
-    trans (interp_rec_pre body (Next (interp_rec body)) env κ).
-    { do 2 f_equiv. rewrite /interp_rec. apply mmuu_unfold. }
-    simpl. rewrite laterO_map_Next. repeat f_equiv.
-    simpl. unfold ir_unf. simpl.
-    intro. simpl. reflexivity.
-  Qed.
-
-  (* Wrong *)
-  Program Definition interp_cont {A}
-    (K : (A -n> (IT -n> IT) -n> IT) -n> (A -n> (IT -n> IT) -n> IT))
-    : A -n> (IT -n> IT) -n> IT
-    := λne env κ, Fun (Next (λne e, K (λne _ _, e) env κ)).
-  Solve All Obligations with try solve_proper.
-  Next Obligation.
-    solve_proper_prepare.
-    repeat f_equiv.
-    by intros ??; simpl.
-  Qed.
-  Next Obligation.
-    solve_proper_prepare.
-    repeat f_equiv.
-    intros ?; simpl.
-    by repeat f_equiv.
-  Qed.
-  Next Obligation.
-    solve_proper_prepare.
-    repeat f_equiv.
-    intros ?; simpl.
-    by repeat f_equiv.
-  Qed.
+  Program Definition interp_throwrk {A} (q : A -n> IT) (K : A -n> (IT -n> IT)) : A -n> (IT -n> IT) := λne env t, interp_throw q (λne env, K env t) env.
+  Solve All Obligations with solve_proper_please.
 
   (** Interpretation for all the syntactic categories: values, expressions, contexts *)
-  Fixpoint interp_val {S} (v : val S) : interp_scope S -n> (IT -n> IT) -n> IT :=
+  Fixpoint interp_val {S} (v : val S) : interp_scope S -n> IT :=
     match v with
     | LitV n => interp_nat n
-    | VarV x => interp_var' x
+    | VarV x => interp_var x
     | RecV e => interp_rec (interp_expr e)
     | ContV K => interp_cont (interp_ectx K)
     end
-  with interp_expr {S} (e : expr S) : interp_scope S -n> (IT -n> IT) -n> IT :=
+  with interp_expr {S} (e : expr S) : interp_scope S -n> IT :=
          match e with
          | Val v => interp_val v
          | App e1 e2 => interp_app (interp_expr e1) (interp_expr e2)
@@ -704,9 +332,9 @@ Section interp.
          | Callcc e => interp_callcc (interp_expr e)
          | Throw e1 e2 => interp_throw (interp_expr e1) (interp_expr e2)
          end
-  with interp_ectx {S} (K : ectx S) : (interp_scope S -n> (IT -n> IT) -n> IT) -n> (interp_scope S -n> (IT -n> IT) -n> IT) :=
+  with interp_ectx {S} (K : ectx S) : interp_scope S -n> (IT -n> IT) :=
          match K with
-         | EmptyK => interp_emptyk
+         | EmptyK => λne env, λne t, t
          | AppLK e1 K => interp_applk (interp_expr e1) (interp_ectx K)
          | AppRK K v2 => interp_apprk (interp_ectx K) (interp_val v2)
          | NatOpLK op e1 K => interp_natoplk op (interp_expr e1) (interp_ectx K)
@@ -718,9 +346,8 @@ Section interp.
          end.
   Solve All Obligations with first [ solve_proper | solve_proper_please ].
 
-  #[global] Instance interp_val_asval {S} (v : val S) (D : interp_scope S)
-   (H : ∀ (x : S), AsVal (D x))
-    : AsVal (interp_val v D idfun).
+  Global Instance interp_val_asval {S} {D : interp_scope S} {H : ∀ (x : S), AsVal (D x)} (v : val S)
+    : AsVal (interp_val v D).
   Proof.
     destruct v; simpl.
     - apply H.
@@ -729,297 +356,308 @@ Section interp.
     - apply _.
   Qed.
 
-  Lemma interp_expr_ren {S S'} env env' κ
-    (δ : S [→] S') (H : env' ≡ (ren_scope δ env)) e :
-    interp_expr (fmap δ e) env κ ≡ interp_expr e env' κ
-  with interp_val_ren {S S'} env env' κ
-    (δ : S [→] S') (H : env' ≡ (ren_scope δ env)) e :
-    interp_val (fmap δ e) env κ ≡ interp_val e env' κ
-  with interp_ectx_ren {S S'} env env' κ φ φ'
-    (δ : S [→] S') (H : env' ≡ (ren_scope δ env)) e :
-    interp_ectx (fmap δ e) φ env κ ≡ interp_ectx e φ' env' κ.
+  Global Instance ArrEquiv {A B : Set} : Equiv (A [→] B) := fun f g => ∀ x, f x = g x.
+
+  Global Instance ArrDist {A B : Set} `{Dist B} : Dist (A [→] B) := fun n => fun f g => ∀ x, f x ≡{n}≡ g x.
+
+  Global Instance ren_scope_proper S S2 :
+    Proper ((≡) ==> (≡) ==> (≡)) (@ren_scope F _ CR S S2).
+  Proof.
+    intros D D' HE s1 s2 Hs.
+    intros x; simpl.
+    f_equiv.
+    - apply Hs.
+    - apply HE.
+ Qed.
+
+  Lemma interp_expr_ren {S S'} env
+    (δ : S [→] S') (e : expr S) :
+    interp_expr (fmap δ e) env ≡ interp_expr e (ren_scope δ env)
+  with interp_val_ren {S S'} env
+         (δ : S [→] S') (e : val S) :
+    interp_val (fmap δ e) env ≡ interp_val e (ren_scope δ env)
+  with interp_ectx_ren {S S'} env
+         (δ : S [→] S') (e : ectx S) :
+    interp_ectx (fmap δ e) env ≡ interp_ectx e (ren_scope δ env).
   Proof.
     - destruct e; simpl.
       + by apply interp_val_ren.
+      + repeat f_equiv; by apply interp_expr_ren.
+      + repeat f_equiv; by apply interp_expr_ren.
+      + repeat f_equiv; by apply interp_expr_ren.
       + f_equiv.
-        * intros ?; by apply interp_expr_ren.
-        * intros ?; simpl; by apply interp_expr_ren.
-      + repeat f_equiv.
-        * intros ?; simpl; by apply interp_expr_ren.
-        * intros ?; simpl; by apply interp_expr_ren.
-      + repeat f_equiv.
-        * intros ?; by apply interp_expr_ren.
-        * intros ?; simpl.
-          repeat f_equiv.
-          -- intros ?; simpl; by apply interp_expr_ren.
-          -- intros ?; simpl; by apply interp_expr_ren.
-      + f_equiv.
-      + repeat f_equiv.
-        intros ?; simpl; by apply interp_expr_ren.
+      + repeat f_equiv; by apply interp_expr_ren.
       + repeat f_equiv.
         intros ?; simpl.
         repeat f_equiv.
-        intros ?; simpl; apply interp_expr_ren.
+        simpl; rewrite interp_expr_ren.
+        f_equiv.
         intros [| y]; simpl.
         * reflexivity.
-        * specialize (H y).
-          apply H.
+        * reflexivity.
       + repeat f_equiv.
         * intros ?; simpl.
-          repeat f_equiv.
-          intros ?; simpl; by apply interp_expr_ren.
-        * intros ?; simpl; by apply interp_expr_ren.
+          repeat f_equiv; first by apply interp_expr_ren.
+          intros ?; simpl.
+          repeat f_equiv; by apply interp_expr_ren.
+        * by apply interp_expr_ren.
     - destruct e; simpl.
-      + f_equiv.
-        rewrite (H _).
-        reflexivity.
       + reflexivity.
-      + clear -interp_expr_ren H.
+      + reflexivity.
+      + clear -interp_expr_ren.
         apply bi.siProp.internal_eq_soundness.
-        iAssert (∀ (S S' : Set) (env : interp_scope S') (env' : interp_scope S) (κ : IT -n> IT) (δ : S [→] S'),
-                   env' ≡ ren_scope δ env -∗ ∀ e : expr S, interp_expr (fmap δ e) env κ ≡ interp_expr e env' κ)%I as "H".
-        {
-          iIntros (? ? ? ? ? ?) "G".
-          iIntros (?).
-          iRewrite "G".
-          iPureIntro.
-          apply interp_expr_ren.
-          reflexivity.
-        }
         iLöb as "IH".
         rewrite {2}interp_rec_unfold.
         rewrite {2}(interp_rec_unfold (interp_expr e)).
-        do 2 iApply f_equivI. iNext.
+        do 1 iApply f_equivI. iNext.
         iApply internal_eq_pointwise.
         rewrite /ir_unf. iIntros (x). simpl.
-        unshelve iApply ("H" $! (inc (inc S)) (inc (inc S')) _ _ κ _ with "[H]").
+        rewrite interp_expr_ren.
+        iApply f_equivI.
         iApply internal_eq_pointwise.
         iIntros (y').
         destruct y' as [| [| y]]; simpl; first done.
         * by iRewrite - "IH".
-        * by rewrite (H _).
+        * done.
       + repeat f_equiv.
         intros ?; simpl; by apply interp_ectx_ren.
-    - admit.
-  Admitted.
-
-  Lemma interp_comp {S} (e : expr S) (env : interp_scope S) (K : ectx S) κ :
-    interp_expr (fill K e) env κ ≡ (interp_ectx K) (interp_expr e) env κ.
-  Proof.
-    revert env.
-    revert κ.
-    induction K; simpl; intros κ env; first reflexivity; try (by rewrite IHK).
-    - f_equiv.
-      intros ?; simpl.
-      by rewrite IHK.
-    - f_equiv.
-      intros ?; simpl.
-      by rewrite IHK.
-    - f_equiv.
-      intros ?; simpl.
-      by rewrite IHK.
+    - destruct e; simpl; intros ?; simpl.
+      + reflexivity.
+      + repeat f_equiv; by apply interp_ectx_ren.
+      + repeat f_equiv; [by apply interp_ectx_ren | by apply interp_expr_ren | by apply interp_expr_ren].
+      + repeat f_equiv; [by apply interp_expr_ren | by apply interp_ectx_ren].
+      + repeat f_equiv; [by apply interp_ectx_ren | by apply interp_val_ren].
+      + repeat f_equiv; [by apply interp_expr_ren | by apply interp_ectx_ren].
+      + repeat f_equiv; [by apply interp_ectx_ren | by apply interp_val_ren].
+      + repeat f_equiv; last by apply interp_expr_ren.
+        intros ?; simpl; repeat f_equiv; first by apply interp_ectx_ren.
+        intros ?; simpl; repeat f_equiv; by apply interp_ectx_ren.
+      + repeat f_equiv; last by apply interp_ectx_ren.
+        intros ?; simpl; repeat f_equiv; first by apply interp_val_ren.
+        intros ?; simpl; repeat f_equiv; by apply interp_val_ren.
   Qed.
 
-  (* Lemma interp_val_push {S} v (env : interp_scope S) κ: *)
-  (*   interp_val v env κ ≡ κ (interp_val v env idfun) *)
-  (* (* with interp_ectx_push {S} k (env : interp_scope S) κ: *) *)
-  (* (*   (λit e : IT, interp_ectx k env κ e) ≡ (κ (λit e : IT, interp_ectx k env idfun e)) *). *)
-  (* Proof. *)
-  (*   { *)
-  (*     destruct v. *)
-  (*     - reflexivity. *)
-  (*     - reflexivity. *)
-  (*     - simpl. *)
-  (*       rewrite !interp_rec_unfold. *)
-  (*       f_equiv. *)
-  (*       simpl. *)
-  (*       repeat f_equiv. *)
-  (*       admit. *)
-  (*     - simpl. *)
-  (*       apply interp_ectx_push. *)
+  Lemma interp_comp {S} (e : expr S) (env : interp_scope S) (K : ectx S):
+    interp_expr (fill K e) env ≡ (interp_ectx K) env ((interp_expr e) env).
+  Proof.
+    revert env.
+    induction K; simpl; intros env; first reflexivity; try (by rewrite IHK).
+    - repeat f_equiv.
+      by rewrite IHK.
+    - repeat f_equiv.
+      by rewrite IHK.
+    - repeat f_equiv.
+      by rewrite IHK.
+    - repeat f_equiv.
+      intros ?; simpl.
+      repeat f_equiv.
+      + by rewrite IHK.
+      + intros ?; simpl.
+        repeat f_equiv.
+        by rewrite IHK.
+  Qed.
 
-  (* Wrong *)
-  (* Program Definition sub_scope {S S'} (δ : S [⇒] S') (env : interp_scope S') *)
-  (*   : interp_scope S := λne x, interp_val (δ x) env idfun. *)
+  Program Definition sub_scope {S S'} (δ : S [⇒] S') (env : interp_scope S')
+    : interp_scope S := λne x, interp_val (δ x) env.
 
-  (* Lemma interp_expr_subst {S S'} (env : interp_scope S') (env' : interp_scope S) κ *)
-  (*   (δ : S [⇒] S') (H : env' ≡ sub_scope δ env) e : *)
-  (*   interp_expr (bind δ e) env κ ≡ interp_expr e env' κ *)
-  (* with interp_val_subst {S S'} (env : interp_scope S') (env' : interp_scope S) κ *)
-  (*        (δ : S [⇒] S') (H : env' ≡ sub_scope δ env) e : *)
-  (*   interp_val (bind δ e) env κ ≡ interp_val e env' κ *)
-  (* with interp_ectx_subst {S S'} (env : interp_scope S') (env' : interp_scope S) κ φ φ' *)
-  (*        (δ : S [⇒] S') (H : env' ≡ sub_scope δ env) e : *)
-  (*   interp_ectx (bind δ e) φ env κ ≡ interp_ectx e φ' env' κ. *)
-  (* Proof. *)
-  (*   - destruct e; simpl. *)
-  (*     + by apply interp_val_subst. *)
-  (*     + f_equiv. *)
-  (*       * intros ?; simpl; by apply interp_expr_subst. *)
-  (*       * intros ?; simpl; by apply interp_expr_subst. *)
-  (*     + f_equiv. *)
-  (*       * intros ?; simpl; by apply interp_expr_subst. *)
-  (*       * intros ?; simpl; by apply interp_expr_subst. *)
-  (*     + f_equiv. *)
-  (*       * intros ?; simpl; by apply interp_expr_subst. *)
-  (*       * intros ?; simpl. *)
-  (*         f_equiv. *)
-  (*         -- f_equiv; by apply interp_expr_subst. *)
-  (*         -- by apply interp_expr_subst. *)
-  (*     + f_equiv. *)
-  (*     + f_equiv. *)
-  (*       intros ?; simpl; by apply interp_expr_subst. *)
-  (*     + repeat f_equiv. *)
-  (*       intros ?; simpl. *)
-  (*       repeat f_equiv. *)
-  (*       intros ?; simpl; apply interp_expr_subst. *)
-  (*       intros [| x']; simpl. *)
-  (*       * reflexivity. *)
-  (*       * rewrite interp_val_ren. *)
-  (*         -- rewrite (H _). *)
-  (*            simpl. *)
-  (*            reflexivity. *)
-  (*         -- intros ?; by term_simpl. *)
-  (*     + repeat f_equiv. *)
-  (*       * intros ?; simpl; by apply interp_expr_subst. *)
-  (*       * intros ?; simpl; by apply interp_expr_subst. *)
-  (*   - destruct e; simpl. *)
-  (*     + term_simpl. *)
-  (*       rewrite (H _). *)
-  (*       simpl. *)
-  (*       admit. *)
-  (*     + reflexivity. *)
-  (*     + clear -interp_expr_subst H. *)
-  (*       apply bi.siProp.internal_eq_soundness. *)
-  (*       iAssert (∀ (S S' : Set) (env : interp_scope S') (env' : interp_scope S) (κ : IT -n> IT) (δ : S [⇒] S'), *)
-  (*                  (env' ≡ sub_scope δ env) -∗ ∀ e : expr S, interp_expr (bind δ e) env κ ≡ interp_expr e env' κ)%I as "H". *)
-  (*       { *)
-  (*         iIntros (? ? ? ? ? ?) "G". *)
-  (*         iIntros (?). *)
-  (*         iRewrite "G". *)
-  (*         iPureIntro. *)
-  (*         apply interp_expr_subst. *)
-  (*         reflexivity. *)
-  (*       } *)
-  (*       iLöb as "IH". *)
-  (*       rewrite {2}interp_rec_unfold. *)
-  (*       rewrite {2}(interp_rec_unfold (interp_expr e)). *)
-  (*       do 2 iApply f_equivI. iNext. *)
-  (*       iApply internal_eq_pointwise. *)
-  (*       rewrite /ir_unf. iIntros (x). simpl. *)
-  (*       unshelve iApply ("H" $! (inc (inc S)) (inc (inc S')) _ _ κ _ with "[H]").         *)
-  (*       iApply internal_eq_pointwise. *)
-  (*       iIntros (y'). *)
-  (*       destruct y' as [| [| y]]; simpl; first done. *)
-  (*       * by iRewrite - "IH". *)
-  (*       * rewrite (H _). *)
-  (*         simpl. *)
-  (*         rewrite interp_val_ren. *)
-  (*         2: reflexivity. *)
-  (*         { *)
-  (*           rewrite interp_val_ren. *)
-  (*           - iPureIntro. reflexivity. *)
-  (*           - intros z; simpl. *)
-  (*             reflexivity. *)
-  (*         } *)
-  (*     + repeat f_equiv. *)
-  (*       intros ?; simpl. *)
-  (*       by apply interp_ectx_subst.         *)
-  (*   - admit. *)
-  (* Admitted. *)
+  Global Instance SubEquiv {A B : Set} : Equiv (A [⇒] B) := fun f g => ∀ x, f x = g x.
+
+  Global Instance sub_scope_proper S S2 :
+    Proper ((≡) ==> (≡) ==> (≡)) (@sub_scope S S2).
+  Proof.
+    intros D D' HE s1 s2 Hs.
+    intros x; simpl.
+    f_equiv.
+    - f_equiv.
+      apply HE.
+    - apply Hs.
+ Qed.
+
+  Lemma interp_expr_subst {S S'} (env : interp_scope S')
+    (δ : S [⇒] S') e :
+    interp_expr (bind δ e) env ≡ interp_expr e (sub_scope δ env)
+  with interp_val_subst {S S'} (env : interp_scope S')
+         (δ : S [⇒] S') e :
+    interp_val (bind δ e) env ≡ interp_val e (sub_scope δ env)
+  with interp_ectx_subst {S S'} (env : interp_scope S')
+         (δ : S [⇒] S') e :
+    interp_ectx (bind δ e) env ≡ interp_ectx e (sub_scope δ env).
+  Proof.
+    - destruct e; simpl.
+      + by apply interp_val_subst.
+      + repeat f_equiv; by apply interp_expr_subst.
+      + repeat f_equiv; by apply interp_expr_subst.
+      + repeat f_equiv; by apply interp_expr_subst.
+      + f_equiv.
+      + repeat f_equiv; by apply interp_expr_subst.
+      + repeat f_equiv.
+        intros ?; simpl.
+        repeat f_equiv.
+        rewrite interp_expr_subst.
+        f_equiv.
+        intros [| x']; simpl.
+        * reflexivity.
+        * rewrite interp_val_ren.
+          f_equiv.
+          intros ?; reflexivity.
+      + repeat f_equiv.
+        * intros ?; simpl.
+          repeat f_equiv; first by apply interp_expr_subst.
+          intros ?; simpl.
+          repeat f_equiv; by apply interp_expr_subst.
+        * by apply interp_expr_subst.
+    - destruct e; simpl.
+      + term_simpl.
+        reflexivity.
+      + reflexivity.
+      + clear -interp_expr_subst.
+        apply bi.siProp.internal_eq_soundness.
+        iLöb as "IH".
+        rewrite {2}interp_rec_unfold.
+        rewrite {2}(interp_rec_unfold (interp_expr e)).
+        do 1 iApply f_equivI. iNext.
+        iApply internal_eq_pointwise.
+        rewrite /ir_unf. iIntros (x). simpl.
+        rewrite interp_expr_subst.
+        iApply f_equivI.
+        iApply internal_eq_pointwise.
+        iIntros (y').
+        destruct y' as [| [| y]]; simpl; first done.
+        * by iRewrite - "IH".
+        * do 2 rewrite interp_val_ren.
+          iApply f_equivI.
+          iApply internal_eq_pointwise.
+          iIntros (z).
+          done.
+      + repeat f_equiv; by apply interp_ectx_subst.
+    - destruct e; simpl; intros ?; simpl.
+      + reflexivity.
+      + repeat f_equiv; by apply interp_ectx_subst.
+      + repeat f_equiv; [by apply interp_ectx_subst | by apply interp_expr_subst | by apply interp_expr_subst].
+      + repeat f_equiv; [by apply interp_expr_subst | by apply interp_ectx_subst].
+      + repeat f_equiv; [by apply interp_ectx_subst | by apply interp_val_subst].
+      + repeat f_equiv; [by apply interp_expr_subst | by apply interp_ectx_subst].
+      + repeat f_equiv; [by apply interp_ectx_subst | by apply interp_val_subst].
+      + repeat f_equiv; last by apply interp_expr_subst.
+        intros ?; simpl; repeat f_equiv; first by apply interp_ectx_subst.
+        intros ?; simpl; repeat f_equiv; by apply interp_ectx_subst.
+      + repeat f_equiv; last by apply interp_ectx_subst.
+        intros ?; simpl; repeat f_equiv; first by apply interp_val_subst.
+        intros ?; simpl; repeat f_equiv; by apply interp_val_subst.
+  Qed.
+
+  (* (** ** Interpretation is a homomorphism *) *)
+  #[global] Instance interp_ectx_item_hom {S} (Ki : ectx S) env :
+    IT_hom (interp_ectx Ki env).
+  Proof.
+    destruct Ki; simpl.
+  Admitted.
 
   (** ** Finally, preservation of reductions *)
-  Lemma interp_expr_head_step {S} env (e : expr S) e' σ σ' K n κ :
+  Lemma interp_expr_head_step {S : Set} (env : interp_scope S) (H : ∀ (x : S), AsVal (env x)) (e : expr S) e' σ σ' K n :
     head_step e σ e' σ' K (n, 0) →
-    interp_expr e env κ ≡ Tick_n n $ interp_expr e' env κ.
+    interp_expr e env ≡ Tick_n n $ interp_expr e' env.
   Proof.
     inversion 1; cbn-[IF APP' INPUT Tick get_ret2].
     - (* app lemma *)
       subst.
-      admit.
-      (* rewrite !interp_expr_subst; [| reflexivity | reflexivity]. *)
-      (* trans (APP (Fun (Next (ir_unf (interp_expr e1) env κ))) (Next $ interp_val v2 env κ)). *)
-      (* + rewrite interp_rec_unfold. *)
-      (*   simpl. *)
-      (*   admit. *)
-      (* + rewrite APP_Fun. simpl. rewrite Tick_eq. do 4 f_equiv. *)
-      (*   intros [| [| x]]; term_simpl. *)
-      (*   * rewrite interp_val_ren. *)
-      (*     -- admit. *)
-      (*     -- reflexivity. *)
-      (*   * admit. *)
-      (*   * reflexivity. *)
+      erewrite APP_APP'_ITV; last apply _.
+      trans (APP (Fun (Next (ir_unf (interp_expr e1) env))) (Next $ interp_val v2 env)).
+      { repeat f_equiv. apply interp_rec_unfold. }
+      rewrite APP_Fun. simpl. rewrite Tick_eq. do 2 f_equiv.
+      simplify_eq.
+      rewrite !interp_expr_subst.
+      f_equiv.
+      intros [| [| x]]; simpl; [| reflexivity | reflexivity].
+      rewrite interp_val_ren.
+      f_equiv.
+      intros ?; simpl; reflexivity.
     - (* the natop stuff *)
       simplify_eq.
       destruct v1,v2; try naive_solver. simpl in *.
       rewrite NATOP_Ret.
       destruct op; simplify_eq/=; done.
-    - subst.
-      rewrite IF_True; last lia.
+    - rewrite IF_True; last lia.
       reflexivity.
-    - subst.
-      rewrite IF_False; last lia.
+    - rewrite IF_False; last lia.
       reflexivity.
-    - subst.
+  Qed.
+
+  Lemma interp_expr_fill_no_reify {S} K (env : interp_scope S) (H : ∀ (x : S), AsVal (env x)) (e e' : expr S) σ σ' n :
+    head_step e σ e' σ' K (n, 0) →
+    interp_expr (fill K e) env ≡ Tick_n n $ interp_expr (fill K e') env.
+  Proof.
+    intros He.
+    trans (interp_ectx K env (interp_expr e env)).
+    { apply interp_comp. }
+    trans (interp_ectx K env (Tick_n n (interp_expr e' env))).
+    {
+      f_equiv. apply (interp_expr_head_step env) in He.
+      - apply He.
+      - apply H.
+    }
+    trans (Tick_n n $ interp_ectx K env (interp_expr e' env)); last first.
+    { f_equiv. symmetry. apply interp_comp. }
+    apply hom_tick_n. apply _.
+  Qed.
+
+  Opaque INPUT OUTPUT_.
+  Opaque Ret.
+
+  Lemma interp_expr_fill_yes_reify {S} K env (e e' : expr S)
+    (σ σ' : stateO) (σr : gState_rest sR_idx rs ♯ IT) n :
+    head_step e σ e' σ' K (n, 1) →
+    reify (gReifiers_sReifier rs)
+      (interp_expr (fill K e) env)  (gState_recomp σr (sR_state σ))
+      ≡ (gState_recomp σr (sR_state σ'), Tick_n n $ interp_expr (fill K e') env).
+  Proof.
+    intros Hst.
+    trans (reify (gReifiers_sReifier rs) (interp_ectx K env (interp_expr e env))
+             (gState_recomp σr (sR_state σ))).
+    { f_equiv. by rewrite interp_comp. }
+    inversion Hst; simplify_eq; cbn-[gState_recomp].
+    - trans (reify (gReifiers_sReifier rs) (INPUT (interp_ectx K env ◎ Ret)) (gState_recomp σr (sR_state σ))).
+      {
+        repeat f_equiv; eauto.
+        rewrite hom_INPUT. f_equiv. by intro.
+      }
+      rewrite reify_vis_eq //; last first.
+      {
+        (* rewrite subReifier_reify/=//. *)
+        (* rewrite H4. done. *)
+        admit.
+      }
+      repeat f_equiv. rewrite Tick_eq/=. repeat f_equiv.
+      rewrite interp_comp.
+      reflexivity.
+    - trans (reify (gReifiers_sReifier rs) (interp_ectx K env (OUTPUT n0)) (gState_recomp σr (sR_state σ))).
+      {
+        do 3 f_equiv; eauto.
+        rewrite get_ret_ret//.
+      }
+      trans (reify (gReifiers_sReifier rs) (OUTPUT_ n0 (interp_ectx K env (Ret 0))) (gState_recomp σr (sR_state σ))).
+      {
+        do 2 f_equiv; eauto.
+        rewrite hom_OUTPUT_//.
+      }
+      rewrite reify_vis_eq //; last first.
+      {
+        (* rewrite subReifier_reify/=//. *)
+        admit.
+      }
+      repeat f_equiv. rewrite Tick_eq/=. repeat f_equiv.
+      rewrite interp_comp.
+      reflexivity.
+    - simpl.
+      rewrite interp_comp.
       admit.
   Admitted.
 
-  (* Lemma interp_expr_fill_no_reify {S} K env (e e' : expr S) σ σ' K n : *)
-  (*   head_step e σ e' σ' K (n, 0) → *)
-  (*   interp_expr (fill K e) env ≡ Tick_n n $ interp_expr (fill K e') env. *)
-  (* Proof. *)
-  (*   intros He. *)
-  (*   trans (interp_ectx K env (interp_expr e env)). *)
-  (*   { apply interp_ectx_fill. } *)
-  (*   trans (interp_ectx K env (Tick_n n (interp_expr e' env))). *)
-  (*   {  f_equiv. apply (interp_expr_head_step env) in He. apply He. } *)
-  (*   trans (Tick_n n $ interp_ectx K env (interp_expr e' env)); last first. *)
-  (*   { f_equiv. symmetry. apply interp_ectx_fill. } *)
-  (*   apply hom_tick_n. apply _. *)
-  (* Qed. *)
-
-  (* Opaque INPUT OUTPUT_. *)
-  (* Opaque Ret. *)
-
-  (* Lemma interp_expr_fill_yes_reify {S} K env (e e' : expr S) *)
-  (*   (σ σ' : stateO) (σr : gState_rest sR_idx rs ♯ IT) n : *)
-  (*   head_step e σ e' σ' (n,1) → *)
-  (*   reify (gReifiers_sReifier rs) *)
-  (*     (interp_expr (fill K e) env)  (gState_recomp σr (sR_state σ)) *)
-  (*     ≡ (gState_recomp σr (sR_state σ'), Tick_n n $ interp_expr (fill K e') env). *)
-  (* Proof. *)
-  (*   intros Hst. *)
-  (*   trans (reify (gReifiers_sReifier rs) (interp_ectx K env (interp_expr e env)) *)
-  (*            (gState_recomp σr (sR_state σ))). *)
-  (*   { f_equiv. by rewrite interp_ectx_fill. } *)
-  (*   inversion Hst; simplify_eq; cbn-[gState_recomp]. *)
-  (*   - trans (reify (gReifiers_sReifier rs) (INPUT (interp_ectx K env ◎ Ret)) (gState_recomp σr (sR_state σ))). *)
-  (*     { repeat f_equiv; eauto. *)
-  (*       rewrite hom_INPUT. f_equiv. by intro. } *)
-  (*     rewrite reify_vis_eq //; last first. *)
-  (*     { rewrite subReifier_reify/=//. *)
-  (*       rewrite H4. done. } *)
-  (*     repeat f_equiv. rewrite Tick_eq/=. repeat f_equiv. *)
-  (*     rewrite interp_ectx_fill. *)
-  (*     by rewrite ofe_iso_21. *)
-  (*   - trans (reify (gReifiers_sReifier rs) (interp_ectx K env (OUTPUT n0)) (gState_recomp σr (sR_state σ))). *)
-  (*     { do 3 f_equiv; eauto. *)
-  (*       rewrite get_ret_ret//. } *)
-  (*     trans (reify (gReifiers_sReifier rs) (OUTPUT_ n0 (interp_ectx K env (Ret 0))) (gState_recomp σr (sR_state σ))). *)
-  (*     { do 2 f_equiv; eauto. *)
-  (*       rewrite hom_OUTPUT_//. } *)
-  (*     rewrite reify_vis_eq //; last first. *)
-  (*     { rewrite subReifier_reify/=//. } *)
-  (*     repeat f_equiv. rewrite Tick_eq/=. repeat f_equiv. *)
-  (*     rewrite interp_ectx_fill. *)
-  (*     simpl. done. *)
-  (* Qed. *)
-
-  Lemma soundness {S} (e1 e2 : expr S) σ1 σ2 (σr : gState_rest sR_idx rs ♯ IT) n m env κ :
+  Lemma soundness {S} (e1 e2 : expr S) σ1 σ2 (σr : gState_rest sR_idx rs ♯ IT) n m (env : interp_scope S) (G : ∀ (x : S), AsVal (env x)) :
     prim_step e1 σ1 e2 σ2 (n,m) →
     ssteps (gReifiers_sReifier rs)
-              (interp_expr e1 env κ) (gState_recomp σr (sR_state σ1))
-              (interp_expr e2 env κ) (gState_recomp σr (sR_state σ2)) n.
+              (interp_expr e1 env) (gState_recomp σr (sR_state σ1))
+              (interp_expr e2 env) (gState_recomp σr (sR_state σ2)) n.
   Proof.
     Opaque gState_decomp gState_recomp.
     inversion 1; simplify_eq/=.
@@ -1027,45 +665,43 @@ Section interp.
       destruct (head_step_io_01 _ _ _ _ _ _ _ H2); subst.
       - assert (σ1 = σ2) as ->.
         { eapply head_step_no_io; eauto. }
-        admit.
-        (* eapply (interp_expr_fill_no_reify K) in H2. *)
-        (* rewrite H2. eapply ssteps_tick_n. *)
+        eapply (interp_expr_fill_no_reify K) in H2; last done.
+        rewrite H2. eapply ssteps_tick_n.
       - inversion H2;subst.
-        + (* eapply (interp_expr_fill_yes_reify K env _ _ _ _ σr) in H2. *)
-          (* rewrite interp_ectx_fill. *)
-          (* rewrite hom_INPUT. *)
-          (* change 1 with (1+0). econstructor; last first. *)
-          (* { apply ssteps_zero; reflexivity. } *)
-          (* eapply sstep_reify. *)
-          (* { Transparent INPUT. unfold INPUT. simpl. *)
-          (*   f_equiv. reflexivity. } *)
-          (* simpl in H2. *)
-          (* rewrite -H2. *)
-          (* repeat f_equiv; eauto. *)
-          (* rewrite interp_ectx_fill hom_INPUT. *)
-          (* eauto. *)
-          admit.
-        + (* eapply (interp_expr_fill_yes_reify K env _ _ _ _ σr) in H2. *)
-          (* rewrite interp_ectx_fill. simpl. *)
-          (* rewrite get_ret_ret. *)
-          (* rewrite hom_OUTPUT_. *)
-          (* change 1 with (1+0). econstructor; last first. *)
-          (* { apply ssteps_zero; reflexivity. } *)
-          (* eapply sstep_reify. *)
-          (* { Transparent OUTPUT_. unfold OUTPUT_. simpl. *)
-          (*   f_equiv. reflexivity. } *)
-          (* simpl in H2. *)
-          (* rewrite -H2. *)
-          (* repeat f_equiv; eauto. *)
-          (* Opaque OUTPUT_. *)
-          (* rewrite interp_ectx_fill /= get_ret_ret hom_OUTPUT_. *)
-          (* eauto. *)
-          admit.
+        + eapply (interp_expr_fill_yes_reify K env _ _ _ _ σr) in H2.
+          rewrite interp_comp.
+          rewrite hom_INPUT.
+          change 1 with (Nat.add 1 0). econstructor; last first.
+          { apply ssteps_zero; reflexivity. }
+          eapply sstep_reify.
+          { Transparent INPUT. unfold INPUT. simpl.
+            f_equiv. reflexivity. }
+          simpl in H2.
+          rewrite -H2.
+          repeat f_equiv; eauto.
+          rewrite interp_comp hom_INPUT.
+          eauto.
+        + eapply (interp_expr_fill_yes_reify K env _ _ _ _ σr) in H2.
+          rewrite interp_comp. simpl.
+          rewrite get_ret_ret.
+          rewrite hom_OUTPUT_.
+          change 1 with (Nat.add 1 0). econstructor; last first.
+          { apply ssteps_zero; reflexivity. }
+          eapply sstep_reify.
+          { Transparent OUTPUT_. unfold OUTPUT_. simpl.
+            f_equiv. reflexivity. }
+          simpl in H2.
+          rewrite -H2.
+          repeat f_equiv; eauto.
+          Opaque OUTPUT_.
+          rewrite interp_comp /= get_ret_ret hom_OUTPUT_.
+          eauto.
+        + admit.
     }
     {
-
+      admit.
     }
-  Qed.
+  Admitted.
 
 End interp.
 #[global] Opaque INPUT OUTPUT_.
